[WIP] associativity of horizontal composition

compcertox/CompCertO.v
@@ -8,7 +8,6 @@ Require Import LanguageInterface_ Events Globalenvs Smallstep_ CategoricalComp F
 Require Import Memory Values.
 Require Import Linking.
 
-(* TODO: move this to compcert *)
 Global Instance fsim_transitive {li1 li2: language_interface}:
   Transitive (forward_simulation (@cc_id li1) (@cc_id li2)).
 Proof.
@@ -97,24 +96,152 @@ Section COMP_FSIM.
 
 End COMP_FSIM.
 
+Require Import SmallstepLinking_.
+
 Section HCOMP_ASSOC.
 
   Context {li} (L1 L2 L3: Smallstep_.semantics li li).
   Variable (sk: AST.program unit unit).
+  Let L12 := fun b => match b with | true => L1 | false => L2 end.
   Let L := fun b => match b with
-                 | true => SmallstepLinking_.semantics
-                            (fun b => match b with | true => L1 | false => L2 end) sk
+                 | true => SmallstepLinking_.semantics L12 sk
                  | false => L3
                  end.
+  Let L23 := fun b => match b with | true => L2 | false => L3 end.
   Let L' := fun b => match b with
                   | true => L1
-                  | false => SmallstepLinking_.semantics
-                              (fun b => match b with | true => L2 | false => L3 end) sk
+                  | false => SmallstepLinking_.semantics L23 sk
                   end.
+
+  Variant frame3: Type :=
+  | fm1: state L1 -> frame3
+  | fm2: state L2 -> frame3
+  | fm3: state L3 -> frame3.
+
+  Inductive flatten1: list (frame L) -> list frame3 -> Prop :=
+  | flatten1_nil_nil: flatten1 nil nil
+  | flatten1_fm1' s k2 k:
+      flatten1 k2 k ->
+      flatten1 (st L true (st L12 true s :: nil) :: k2) (fm1 s :: k)
+  | flatten1_fm1 s k1 k2 k:
+      k1 <> nil -> flatten1 (st L true k1 :: k2) k ->
+      flatten1 (st L true (st L12 true s :: k1) :: k2) (fm1 s :: k)
+  | flatten1_fm2' s k2 k:
+      flatten1 k2 k ->
+      flatten1 (st L true (st L12 false s :: nil) :: k2) (fm2 s :: k)
+  | flatten1_fm2 s k1 k2 k:
+      k1 <> nil -> flatten1 (st L true k1 :: k2) k ->
+      flatten1 (st L true (st L12 false s :: k1) :: k2) (fm2 s :: k)
+  | flatten1_fm3 s k1 k:
+      flatten1 k1 k ->
+      flatten1 (st L false s :: k1) (fm3 s :: k).
+
+  Inductive flatten2: list (frame L') -> list frame3 -> Prop :=
+  | flatten2_nil_nil: flatten2 nil nil
+  | flatten2_fm1 s k1 k:
+      flatten2 k1 k ->
+      flatten2 (st L' true s :: k1) (fm1 s :: k)
+  | flatten2_fm2' s k2 k:
+      flatten2 k2 k ->
+      flatten2 (st L' false (st L23 true s :: nil) :: k2) (fm2 s :: k)
+  | flatten2_fm2 s k1 k2 k:
+      k1 <> nil -> flatten2 (st L' false k1 :: k2) k ->
+      flatten2 (st L' false (st L23 true s :: k1) :: k2) (fm2 s :: k)
+  | flatten2_fm3' s k2 k:
+      flatten2 k2 k ->
+      flatten2 (st L' false (st L23 false s :: nil) :: k2) (fm3 s :: k)
+  | flatten2_fm3 s k1 k2 k:
+      k1 <> nil -> flatten2 (st L' false k1 :: k2) k ->
+      flatten2 (st L' false (st L23 false s :: k1) :: k2) (fm3 s :: k).
+
+  Hint Constructors flatten1 flatten2.
+
+  Definition state_match (s1: list (frame L)) (s2: list (frame L')): Prop :=
+    exists fm, flatten1 s1 fm /\ flatten2 s2 fm.
 
   Lemma horizontal_compose_associativity:
     SmallstepLinking_.semantics L sk ≤ SmallstepLinking_.semantics L' sk.
   Proof.
+    constructor. econstructor. reflexivity.
+    intros. apply or_assoc.
+    intros se ? [ ] qset [ ] Hse.
+    instantiate (1 := fun _ _ _ => _). cbn beta.
+    apply forward_simulation_step
+      with (match_states := state_match); cbn.
+    - intros q ? s1 <- H. inv H. destruct i.
+      (* initial state of L12 *)
+      + cbn in *. inv H1. destruct i.
+        (* initial state of L1 *)
+        * cbn in *. eexists; split.
+          apply initial_state_intro with (i := true).
+          firstorder. eauto.
+          eexists. split; eauto.
+        (* initial state of L2 *)
+        * cbn in *. eexists; split.
+          apply initial_state_intro with (i := false).
+          cbn. firstorder.
+          apply initial_state_intro with (i := true).
+          firstorder. eauto.
+          eexists. split; eauto.
+      (* initial state of L3 *)
+      + cbn in *. eexists; split.
+        apply initial_state_intro with (i := false).
+        cbn. firstorder.
+        apply initial_state_intro with (i := false).
+        firstorder. eauto.
+        eexists. split; eauto.
+    - intros s1 s2 r Hs H. exists r; split; auto.
+      inv H. destruct i.
+      (* final state of L12 *)
+      + cbn in *. inv H0. destruct i.
+        (* final state of L1 *)
+        * cbn in *. destruct Hs as [fs [Hs1 Hs2]].
+          admit.
+        (* final state of L2 *)
+        * admit.
+      (* final state of L3 *)
+      + cbn in *. destruct Hs as [fs [Hs1 Hs2]].
+        inv Hs1. subst_dep.
+        inv H3. inv Hs2. inv H2.
+        repeat constructor; auto.
+        inv H4.
+    - admit.
+    - intros s1 t s1' Hstep s2 Hs.
+      inv Hstep.
+      (* internal step *)
+      + destruct i.
+        (* internal step of L12 *)
+        * inv H.
+          (* internal step of L1 or L2 *)
+          {
+            destruct i.
+            (* internal step of L1 *)
+            - destruct Hs as [fm [Hs1 Hs2]].
+              inv Hs1.
+              inv Hs.
+              admit.
+            (* internal step of L2 *)
+            - admit.
+          }
+          (* cross component call between L1 and L2 *)
+          -- admit.
+          (* return *)
+          -- admit.
+        (* internal step of L3 *)
+        * admit.
+      (* cross component call between L12 and L3 *)
+      + destruct i.
+        (* call from L12 *)
+        * cbn in *. inv H. destruct i.
+          (* call from L1 *)
+          -- admit.
+          (* call from L2 *)
+          -- admit.
+        (* call from L3 *)
+        * admit.
+      (* return *)
+      + admit.
+
   Admitted.
 
 End HCOMP_ASSOC.
